**Problem 67**: $(a+b)(a-b) = a(a-b)+b(a-b) = a^2-ab+ab-b^2 = a^2-b^2$


**Problem 68**: $101 \cdot 99 = (100+1)(100-1) = 100^2-1^2 = 10000-1 = 9999$


**Problem 69**: You cut the rectangle whose lengths are $b$ and $a-b$ to the top and you get a rectangle that is $a+b$ by $a-b$. 


**Problem 70**: $x\cdot (x+2)+1 = x^2 + 2x + 1 = (x+1)^2$



**Problem 71**: So you have $n^2$ and $(n+1)^2$, so the difference is $2n+1$, and using that $2n+1$ you get every odd number.


**Problem 72**: $(n5)^2 = (10n+5)^2 = 100n^2+100n+25 = 100(n(n+1))+25$, and you can see that the part with the $n$'s, its $n(n+1)25$.


**Problem 73**: $(a+b+c) = (a+b+c)(a+b+c) = a^2+ab+ac+ab+b^2+bc+ac+bc+c^2=
a^2+b^2+c^2+2ab+2ac+2bc$


**Problem 74**: $(a+b-c)^2 = (a+b+(-c))^2$, then you just put the $-c$ into the previous equation, $a^2+b^2+c^2+2ab-2ac-2bc$


**Problem 75**: $(a+b+c)(a+b-c) = ((a+b)+c)((a+b)-c) = (a+b)^2 - c^2 = a^2 + 2ab + b^2 - c^2$


**Problem 76**: ($\textcolor{red}{Wrong}$) $(a+b+c)(a-b-c) = (a+(b+c))(a-(b+c)) = a^2-(b+c)^2 = a^2-b^2+2bc+c^2$


**Problem 77**: ($\textcolor{red}{Wrong}$) $(a+b-c)(a-b+c) = (a+(b-c))(a-(b-c)) = a^2-(b-c)^2 = a^2 - b^2 - 2bc+c^2$


**Problem 78**:$(a^2-2ab+b^2)(a+2ab+b^2) = (a-b)^2(a+b)^2 = ((a-b)(a+b))^2 = (a^2-b^2)^2 = a^4-2a^2b^2+b^4$ 


**Problem 79**: $11^3 = (10+1)^3 = 1000+300+30+1 = 1331$


**Problem 80**: $101^3 = (100+1)^2 = 1000000+30000+300+1 = 1030301$


**Problem 81**: $(a-b)^3 = (a+(-b))^3 = a^3-3a^2b+3ab^2-b^3$


**Problem 82**: 
* $11^3 = (10+1)^3 = 1000+300+3+1 = 1331$
* $11^4 = (10+1)^4 = 10000+4000+600+40+1 = 14641$
* $11^5= (10+1)^5 = 100000+50000+10000+1000+50+1 = 161051$ 
* $11^6 = (10+1)^5 = 1000000+600000+150000+20000+1500+60+1 = 1771561$ $


**Problem 83**: $(a+b)^7 = a^7 + 7a^6b+21a^5b^2+ 35a^4b^3+35a^3b^4 + 21a^2b^5+ 7ab^6+b^7$


**Problem 84**: 
* $(a-b)^4 = (a+(-b))^4 = a^4-4a^3b+6a^2b^2-4ab^3+b^4$
* $(a-b)^5 = (a+(-b))^5 = a^5-5a^4b+10a^3b^2-10a^2b^3+5ab^4-b^5$
* $(a-b)^6 = (a+(-b))^6 = a^6-6a^5b+15a^4b^2-20a^3b^3+15a^2b^3-6ab^5+b^6$


**Problem 85**: First row: $1$, second row: $2$, third row: $4$. You can see that it multiplies my two each time. 


**Problem 86**: 
* $(a+a)^2 = (2a)^2 = 4a^2$
* $(a+a)^3 = (2a)^3 = 8a^3$
* $(a+a)^4 = (2a)^4 = 16a^4$


**Problem 87**: They both the powers of 2. When $a=1$, problem 86 reduces to problem 85.


**Problem 88**: 
* $(-b+b)^2 = 0^2 = 0$
* $(-b+b)^3 = 0$
* $(-b+b)^4 = 0$


**Problem 89**: $(1+x-y)(12-zx-y) = 12-zx-y+12x-xzx-xy-12y+yzx+y^2 = 12-xy-13y+12x-x^2z-xy+xyz+y^2$


**Problem 90**: 
* $(1+x)(1+x^2) = 1+x^2 + x + x^3 = x^3+x^2+x+1$
* ($\textcolor{red}{Wrong}$) $(1+x)(1+x^2)(1+x^4)(1+x^8) = ((1+x)(1+x^2))(1+x^4)(1+x^8) =  (1+x+x^2+x^3)(1+x^4) = 1+x+x^2+x^3+x^4+x^5+x^6+x^7 = 1+x+x^2+x^3+x^4+x^5+x^6+x^7 (1+x^8) = 1+x+x^2+x^3+x^4+x^5+x^6+x^7+x^8+x^9+x^{10}+x^{11}+x^{12}+x^{13}+x^{14}+x^{15}$
* $(a+b+c+d)^2 = a^2+b^2+c^2+d^2+2ab+2ac+2ad+2bc+2bd+2cd$, So $(1+x+x^2+x^3)^2 = 1+x^2+x^4+x^6+2x+2x^2+2x^3+2x^3+2x^4+2x^5 = 1+ 2x+3x^2+4x^3+3x^4+2x^5+x^6$
* $(1+x+x^2+x^3\cdots+x^9+x^{10})^2$, You can see that there is a pattern in the coefficients, which is the ocefficients go up and down, so you can get $1+2x+ 3x^2+4x^3+5x^4+6x^5+7x^6+8x^7+9x^8+10x^9+11x^{10}+10x^{11}+9x^{12}+8x^{13}+7x^{ 14}+6x^{15}+5x^{16}+4x^{17}+3x^{18}+2x^{19}+x^{20}$ 
* ($\textcolor{red}{Wrong}$) Since the only way you can get $x^{30}$ is from the $(x^10)^3$, so the coefficient for $x^{30}$ in this equation would be $1$. For $x^29$, there are also only one because the only way you can get it is from the $x^9\cdot x^10\cdot x^10$, which has three different ways to order them, so the coefficient for $x^{29}$ is equal to three.
* ($\textcolor{red}{calculate this explicitly}$)If you take $(1-x)(1+x)$ for example, you get $1-x^2$ as an answer. If you do $(1-x)(1+x+x^2)$ you get $1-x^3$, and you can start to see a pattern. So for $(1-x)(1+x+x^2+\cdot +x^9+x^{10})$ you get $1-x^{11}$
* $(a+b)(a^2-ab+b^2)= a^3-a^2b+ab^2+a^2b-ab^2+b^3 = a^3+b^3$
* I don't have an answer for this.




**Problem 99**: The solution is in the book: $1$, $1+1$, $1+2+1$, $1+3+3+1$, $\cdots$


**Problem 100**: $(1+(-1))^2 = 0^2 = 0$


**Problem 101**: ($\textcolor{red}{Wrong}$) So you take $x=1$ then you have $(1+2x)^{200} =$ some coefficients plus one, so it will be $2^{200} -1$.


**Problem 102**: ($\textcolor{red}{Wrong}$) If you take $x=1$, you get $(1-2)^200 = (-1)^200 = 1$ 


**Problem 103**: If you expand it you get $1+3x-3y-6xy+3y^2+3x^2+x^3-3x^2y+3xy^2-y^3$, and if you do $x=1$ you get $1$.


**Problem 104**: ($\textcolor{red}{Wrong}$)If $x=1$, then $1+3x+3x^2+x^3$ which has a coefficient sum of $8$.


**Problem 105**: ($\textcolor{red}{Wrong}$)If $x=1$ then you get $3x-6xy+3x^2+x^3-3x^2y+3xy^2$ and the coefficient sum is $1$. 


