**Problem 253**: So you start with $ax^2+bx+c=0$, so you first divide that by $x^2$ and you get $a+\frac{b}{x}+\frac{c}{x^2}=0$, then you turn that into $c\cdot (\frac{1}{x})^2+b\cdot (\frac{1}{x})^2+a=0$. So the roots for $cx^2+bx+a=0$ would equal to $\frac{1}{x_1}$ and $\frac{1}{x_2}$ 


**Problem 254**: Using the cross multiplication method, I solved for the 2 possible outcomes:

$$\frac{-b + \sqrt{b^2-4ac}}{2a}= \frac{2c }{-b-\sqrt{b^2-4ac}}$$

Then I used the cross multiplication method:

$$2a\cdot2c=(-b+\sqrt{b^2-4ac})(-b-\sqrt{b^2-4ac})$$
$$4ac=b^2+b(\sqrt{b^2-4ac})-b(\sqrt{b^2-4ac})-(\sqrt{b^2-4ac})^2$$
$$4ac=b^2-b^2+4ac$$
$$4ac=4ac$$

Now for the other possiblitily, it will be the same because it will change the equation from 

$$2a\cdot2c=(-b+\sqrt{b^2-4ac})(-b-\sqrt{b^2-4ac})$$

to

$$2a\cdot2c=(-b-\sqrt{b^2-4ac})(-b+\sqrt{b^2-4ac})$$

**Problem 255**: No because when $a=0$ the equaltion isn't quadratic anymore, so it will only have one root.


**Problem 256**: For question $a$, I first found that to find the delta, which is $1+4a$, 
* $\Delta=4a+1>0$, then there are two roots and $a>-\frac{1}{4}$
* $\Delta=4a+1=0$ then there is one root and $a=\frac{1}{4}$
* $\Delta=4a+1<0$ then there are no roots and $a<-\frac{1}{4}$.

For question $b$, I did the same thing as problem $a$, find $\Delta$, which is $b^2-4ac$ or in this question it would be $a^2-4$.
* $\Delta=a^2-4>0$, then there are two roots and $a>2$ and $a<-2$
* $\Delta=a^2-4=0$ then there is one root and $a=\pm2$
* $\Delta=a^2-4<0$ then there are no roots and $a<2$ and $a>-2$


**Problem 257**: The coordinates are $(-m, n)$ because the $m$ value moves it left or right while the $n$ value moves the point up or down.


**Problem 258**: Ordering the operation is important because if you do it a differnet way, then the equation is wrong. For example if you do $c$ then $b$ then $a$, your final equation is $a(x+m)^2+an$, not $a(x+m)^2+n$.


**Problem 259**: 
first (b) applying $x+m$ and c vertical shift $+n$ are commutative. so we have 
* abc=acb, which is $a(x+m)^2+n$.
* similarly, bca=cba, which is $a(x+m)^2+an$.
* the remaining bac is $a(x+m)^2+n$ and cab is $a(x+m)^2+an$.

So we have two forms:
* abc=acb=bac (a must be before c) leads to $a(x+m)^2+n$
* cab=cba=bca (a must be before a) leads to $a(x+m)^2+an$


**Problem 260**: If the parabola is facing up, then $a$ would be positive. If it's negative, then it's facing downwards. To find the sign of $\frac{b}{a}$, it would be the vertex of the parabola. For the sign of $c$ then it is the interesection of the graph and the y-axis.


**Problem 261**: So if you factor $x^2-3x+2$ you get $(x-2)(x-1)$, so if you were to draw that out it would look like a number line and all the numbers that satisfy this: $1<x<2$ both factors are negative and any other number both factors are positive.


**Problem 262**: Say that one of the number is $x$, then the other number must be $1-x$. So you multiply them together and you get $x\cdot(1-x)=x-x^2=-x^2+x$. So if you were to graph $-x^2+x$ then it would be a parabola facing down and the roots of it would be $1$ and $0$. So the vertex would be $\frac{1}{2}$, and by putting that back into the first equation you get $\frac{1}{2}\cdot(1-\frac{1}{2})=\frac{1}{4}$


**Problem 263**: So say that the side of the square is $s$, then the perimeter of that square would be $4s$, and a rectangle with the same perimeter would be $2(s+x)+2(s-x)$, ($x$ is an interger). So the area for the square would be $s^2$ and the area for the rectangle would be $(s+x)(s-x)=s^2-x^2$, so the square's area is greater than a rectangle with the same perimeter.


**Problem 264**: So using the solution for problem 265, you can generalize the formula to the minimal of $x+\frac{s}{x}$ for positive $x$ is $2\sqrt{s}$ when $x=\sqrt{s}$. So assume that the sides of the rectangle is $a$ and $b$, and the area is $s$, then the minimal of $a+b$ or $a+\frac{s}{a}$ would be when $a=\sqrt{s}$, and $b$ is equal to $\frac{s}{a}$, then $b$ is also equal to $\sqrt{s}$, so $a=b$, which means that it is a square.


**Problem 265**: So say that $c$ is equal to $x+\frac{2}{x}$. So if you multiply the equation by $x$, then you get $x^2+2=cx$, which can be rewritten as $x^2-cx+2=0$, which you can see is a quadratic equation. Since it's a quadratic equation, it has solution when the discrimiant is nonnegative, so the equation would be $D=(\frac{c}{2})^2-2$. Using that you can rewrite it as $(\frac{c}{2})^2 \ge 2$. So $\frac{c}{2}\ge \sqrt{2}$ or $\frac{c}{2}\le \sqrt{2}$. So the minimun value would be for positive $x$, $2\sqrt{2}$


**Problem 266**: Assume that $y=x^2$. Then you change the equation from $x^4-3x^2+2=0$ to $y^2-3y+2=0$. So using that you can plug that into the quadratic equation, which makes it $y=\frac{3\pm\sqrt{9-8}}{2}=\frac{3\pm1}{2}$, so $y=1$ and $2$. Using that info you know that $x^2=1$ and $x^2=2$, so there are four solution for $x$, $1$, $-1$, $\sqrt{2}$, and $-\sqrt{2}$




**Problem 267**: For the next six problems, $y$ is always equal to $x^2$.
* For no solution, I just need an equation in which it is simplified it is $x^4$ is equal to a negative number, so I made $x^4+2=0$
* For one solution, you can do $x^4=0$, which only has one solution, which is $0$
* For two solutions, I did $x^4-1=0$, which is equal to $x^4=1$, so the two solutions are $1$ and $-1$
* $x^4-2y^2+0=0$, which is equal to $y^2-2y+0=0$, which factorized is $(y-2)(y-0)$. So there are three solutions for $x$, $\sqrt{2}$, $-\sqrt{2}$, and $0$
* You can use the equation from problem 266 or you can use this: $x^4-4x^2+3=0$ which is equal to $y^2-4y+3=0$ which equals to $(x-1)(x-3)$ so the solution is $1$ and $3$, so if you take those numbers and square root them to find $x$ values, which are $1$, $-1$, $\sqrt{3}$, and $-\sqrt{3}$
* So in a biquadratic equation the maxium number of answers (excluding infinity) is four, so a biquadratic equation that has exaclty five solution cannot be possible. (See Problem 148)




**Problem 268**: So I first did $y=x^3$ so that I can change the equation from $ax^6+bx^3+c=0$ to $ay^2+by+c=0$. From that $y$ can have zero, one, or two possible answer (because it is a quadratic equation). So $x=\sqrt[3]{y}$ can have up to two solutions. But the hint said that $a$, $b$, or $c$ could be equal to $0$, so if you assume that $a$, $b$, and $c$ are all zeros, then there are infinite possiblilities because any number can be $x$ and the equation would still work. 




**Problem 269**: 

* Assume that $y=x^4$, then you can rewrite $ax^8+bx^4+c=0$ to $ay^2+by+c=0$. 
* if $\Delta<0$, then $y$ has no solution so does $x$.
* If there is one answer for the quadratic equation $ay^2+by+c=0$, say it's $y_0$. 
    * if $y_0<0$, then no solution
    * if $y_0=0$, then one solution
    * if $y_0>0$, then $y=x^4$. So $x^2=\pm\sqrt{y}$. So there two possible solutions.  
* So then I assumed that there are 2 answers for the quadratic equation $ay^2+by+c=0$. 
    * $y_1,y_2>0$, there are $4$ solutions.
    * $y_1=0,y_2>0$, there are $3$ solutions.
    * $y_1<0,y_2>0$, there are $2$ solutions.
    * $y_1<0,y_2=0$, there are $1$ solution.
    * $y_1<0,y_2<0$, there are $0$ solutions. 

* So right now $ax^8+bx^4+c=0$ could have up to four possible answers or infinitely many answers. 




**Problem 270**: So I first divided that equation by $x^2$, and I got $2x^2+7x+4+\frac{7}{x}+\frac{2}{x^2}=0$. And then I rewrote it as $2(x^2+\frac{1}{x^2})+7(x+\frac{1}{x})+4=0$. Then I used the $x^2+\frac{1}{x^2}$ which can be expressed in terms of $x+\frac{1}{x}$, so I did $(x+\frac{1}{x})^2=x^2+2\cdot x\cdot\frac{1}{x}+(\frac{1}{x})^2=x^2+\frac{1}{x^2}+2$ so $x^2+\frac{1}{x^2}=(x+\frac{1}{x})^2-2$. Since $x$ is a solution of the equation then I found that if $y=x+\frac{1}{x}$ then there is a solution for the equation $2(y^2-2)+7y+4=0$ and $2y^2-4+7y+4=0$ or $2y^2+7y=0$ or $y(2y+7)=0$. And the solution for those equation is $y=0$ and $-\frac{7}{2}$. So that means $x+\frac{1}{x}=0$ and $-\frac{7}{2}$. So for the first equation, $x+\frac{1}{x}=0$ there are no solution because if you simplify it it becomes $x^2=-1$, which is impossible. For the second equation, $x+\frac{1}{x}=-\frac{7}{2}$, you can simplify it to $x^2+1=-\frac{7}{2}x$ which is equal to $x^2+\frac{7}{2}x+1=0$, which is a quadratic equation. So using the quadratic equation you get $x_{1,2}=\frac{-\frac{7}{2}\pm \sqrt{\frac{49}{4}-4}}{2}=\frac{\frac{-7}{2}\pm \frac{\sqrt{33}}{2}}{2}$. So $x_1$ and $x_2$ is equal to $\frac{-7+\sqrt{33}}{4}$ and $\frac{-7-\sqrt{33}}{4}$






