**Problem 106**: $ac+ad+bc+bd=(a+b)(c+d)$

**Problem 107**: 
* $ac+bc-ad-bd=a(c-d)+b(c-d)=(a+b)(c-d)$
* $1+a+a^2+a^3=(a+1)(a^2+1)$
* $1+a+a^2+\cdots+a^{14}=(1+a+a^2+a^3+a^4)(a^5+a^6+a^7+a^8+a^9)(a^{10}+a^{11}+a^{12}+a^{13}+a^{14})=(1+a+a^2+a^3+a^4)+a^5(1+a+a^2+a^3+a^4)+a^10(1+a+a^2+a^3+a^4)=(1+a^5+a^{10})(1+a+a^2+a^3+a^4)$
* $x^4-x^3+2x-2=(x-1)(x^3+2)$

**Problem 108**: $(a+2b)(a+b)$

**Problem 109**: 
* $a^2-3ab+2b^2=a^2-ab-2ab+2b^2=a(a-b)-2b(a-b)=(a-b)(a-2b)$
* $a^2+3a+2=a^2+2a+a+2=a(a+2)+a+2=(a+2)(a+1)$

**Problem 110**: 
* $a^2+4ab+4b^2=(a+2b)^2$
* $a^4+2a^2b^2+b^4=(a^2)^2+2a^2b^2+(b^2)^2=(a^2+b^2)^2$
* $a^2-2a+1=(a-1)^2$

**Problem 111**: $x^5+x+1=x^5+x^4+x^3-x^4-x^3-x^2+x^2+x+1=x^3(x^2+x+1)-x^2(x^2+x+1)+(x^2+x+1)=(x^3-x^2+1)(x^2+x+1)$

**Problem 112**: $a^2=b^2$, so $a^2-b^2=0$ which equals to $(a+b)(a-b)=0$, so either $a=b$ or $a=-b$.


**Problem 113**: $a^3-b^3=a^3-a^2b+a^2b-ab^2+ab^2-b^3=a^2(a-b)+ab(a-b)+b^2(a-b)=(a^2+ab+b^2)(a-b)$

**Problem 114**: $a^3+b^3=a^3+a^2b-a^2b+ab^2-ab^2+b^3=a^2(a+b)-ab(a+b)+b^2(a+b)=(a^2-ab+b^2)(a+b)$

**Problem 115**: $a^4-b^4=a^4-a^3b+a^3b-a^2b^2+a^2b^2-ab^3+ab^3-b^4=a^3(a-b)+a^2b(a-b)+ab^2(a-b)+b^3(a-b)=(a-b)(a^3+a^2b+ab^2+b^3)$

**Problem 116**: 
* $a^5-b^5=(a-b)(a^4+a^3b+a^2b^2+ab^3+b^4)$
* $a^{10}-b^{10}=(a-b)(a^9+a^8b+a^7b^2+a^6b^3+a^5b^4+a^4b^5+a^3b^6+a^2b^7+ab^8+b^9)$
* $a^7-1=(a-1)(a^6+a^5+a^4+a^3+a^2+a+1)$

**Problem 117**: $a^2-4b^2=a^2-2^2b^2=a^2-(2b^2)=(a-2b)(a+2b)$

**Problem 118**: 
* $a^2-2=(a+\sqrt{2})(a-\sqrt{2})$
* $a^2-3b^2=(a+\sqrt{3}b)(a-\sqrt{3}b)$
* $a^2+2ab+b^2-c^2=(a+b)^2-c^2=(a+b-c)(a+b+c)$
* $a^2+4ab+3b^2=(a^2+ab)(3ab+3b^2)=a(a+b)+3b(a+b)=(a+b)(a+3b)$

**Problem 119**: $a^4+b^4=a^4+2a^2b^2+b^4-2a^2b^2=(a^2+b^2)^2-(\sqrt{2}ab)^2=(a^2+b^2+\sqrt{2}ab)(a^2+b^2-\sqrt{2}ab)$

**Problem 120**: skip

**Problem 121**: $(2+3\sqrt{-1})(2-3\sqrt{-1})=2^2-(3\sqrt{-1})^2=4+9=13$

**Problem 122**: 
* $x^4+1=(x^4+2x^2+1)-2x^2=(x^2+1)^2-2x^2=(x^2+\sqrt{2}x+1)(x^2-\sqrt{2}x+1)$
* $$x(y^2-z^2)+y(z^2-x^2)+z(x^2-y^2)$$

$$=xy^2-xz^2+yz^2-x^2y+x^2z-y^2z$$

$$=x(y^2-z^2)+yz(z-y)+x^2(z-y)$$

$$=x(y-z)(y+z)+yz(z-y)+x^2(z-y)$$

$$=(y-z)(x(y+z)-yz-x^2)=(y-z)(x(y-x)-z(y-x))=(y-z)(y-x)(x-z)$$
* $a^{10}+a^5+1=(a^2+a+1)(a^8-a^7+a^5-a^4+a^3-a+1)$
* $a^3+b^3+c^3-3abc=(a+b+c)(a^2+b^2+c^2-ab-bc-ac)$
* $(a+b+c)^3-a^3-b^3-c^3=3a^2b+3ab^2+3a^2c+3ac^2+3b^2c+3bc^2+6abc=3(a^2b+ab^2+a^2c+ac^2+b^2c+bc^2+2abc)=3(a^2(b+c)+a(b^2+c^2+2bc)+bc(b+c))=3(a^2(b+c)+a(b+c)^2+bc(b+c))=3(b+c)(a^2+ab+ac+ab)=3(a+b)(a+c)(b+c)$
* $a^3-3a^2b+3ab^2-b^3+b^3-3b^2c+3bc^2-c^3+c^3-3c^2a+3ca^2-a^3=-3a^2b+3ab^2-3b^2c+3bc^2+3a^2c-3ac^2=-3(a^2b-ab^2+b^2c-bc^2-a^2c+ac^2)=-3(a^2(b-c)-a(b^2-c^2)+bc(b-c))=-3(a^2(b-c)-a(b-c)(b+c)+bc(b-c))=-3((b-c)(a^2-ab-ac+bc))=-3(b-c)(a-b)(a-c)$

**Problem 123**: 
$$a+b<1+ab$$
$$0<(1+ab)-(a+b)$$
$$0<(a-1)(b-1)$$

So since $a$ and $b$ are both greater than $1$ then that means $a-1$ times $b-1$ will always be greater than $0$.

**Problem 124**: First, you can turn $a^2+ab+b^2=0$ into $a^3-b^3=0$ (because $a^3-b^3$ is divisible by $a^2+ab+b^2$). Then you have $a^3-b^3=(a-b)(a^2+ab+b^2)=0$,so that means $a=b$. Now if you plug $a=b$ into $a^2+ab+b^2=0$ and you get $3a^2=0$, so $a^2=0$, so $a$ and $b$ both must equal to $0$.

**Problem 125**: By using $a^3+b^3+c^3-3abc=(a+b+c)(a^2+b^2+c^2-ab-bc-ac)$ formula, if $a+b+c=0$ then the left side also equals $0$, so $a^3+b^3+c^3=3abc$

**Problem 126**: 
$$\frac{1}{a+b+c}=\frac{ab+ac+bc}{abc}$$
$$=abc=(a+b+c)(ab+ac+bc)=abc+a^2c+a^2b+b^2c+abc+ab^2+bc^2+ac^2+abc$$
$$0=2abc+a^2c+a^2b+b^2c+ab^2+bc^2+ac^2$$
$$0=(a+b)(b+c)(c+a)$$

So from that there must be two opposite numbers because either $a+b$, $b+c$, or $c+a$ must be equal to $0$.


**Problem 127**: 
* $(a)$: $\frac{ab}{c}$
* $(b)$: $\frac{ac}{b^2}$
* $(c)$: $\frac{x}{x+1}$
* $(d)$: $\frac{2x+1}{3x+2}$
* $(e)$: $\frac{x^2z+y^2x+z^2y+y^2z+z^2x+x^2y}{y^2z+z^2x+x^2y}$
* $(f)$: $\frac{x^3+x^2+x+1}{x+1}=x^2+1$
* $(g)$: $\frac{2ab}{a+b}$

**Problem 128**: $\frac{(x-a)(x-b)}{(c-a)(c-b)}+\frac{(x-a)(x-c)}{(b-a)(b-c)}+\frac{(x-b)(x-c)}{(a-b)(a-c)}=1$

**Problem 129**: 
* $x=a$: $\frac{(a-a)(a-b)}{(c-a)(c-b)}+\frac{(a-a)(a-c)}{(b-a)(b-c)}+\frac{(a-b)(a-c)}{(a-b)(a-c)}=\frac{(a-b)(a-c)}{(a-b)(a-c)}=1$
* $x=b$: $\frac{(b-a)(b-b)}{(c-a)(c-b)}+\frac{(b-a)(b-c)}{(b-a)(b-c)}+\frac{(b-b)(b-c)}{(a-b)(a-c)}=1$
* $x=c$: $\frac{(c-a)(c-b)}{(c-a)(c-b)}+\frac{(c-a)(c-c)}{(b-a)(b-c)}+\frac{(c-b)(c-c)}{(a-b)(a-c)}=1$

**Problem 130**: Just by using the harmonic mean formula you can find the answer, which is $\frac{1}{(\frac{1}{a}+\frac{1}{b})\cdot \frac{1}{2}}$

**Problem 131**: Assume $x$ is the boat's speed and $y$ is the current's speed. Then you have $\frac{1}{x+y}=a$ hours and $\frac{1}{x-y}=b$ hours, and you need to find what $\frac{1}{x}$ is. So you have $x+y=\frac{1}{a}$ and $x-y=\frac{1}{b}$, then you do $2x=\frac{1}{a}+\frac{1}{b}$, so you find that $\frac{1}{x}=\frac{2}{\frac{1}{a}+\frac{1}{b}}$

**Problem 132**: Assume the distance they are driving is one mile, then you have for the first half mile they drove at $\frac{1}{v_1}$ miles per hour and then they drove the second half mile at $\frac{1}{v_1}$ miles per hour. So they drove a total of $\frac{1}{\frac{1}{2v_1}+\frac{1}{2v_2}}$

**Problem 133**: 
* $x^2+\frac{1}{x^2}=$
$$x+\frac{1}{x}=7$$
$$x^2+2\cdot x \cdot \frac{1}{x}+\frac{1}{x^2}=49$$
$$x^2+2+\frac{1}{x^2}=49$$
$$x^2+\frac{1}{x^2}=47$$
* $x^3+\frac{1}{x^3}=$

$$x^3+3x^2\cdot \frac{1}{x}+3x\cdot \frac{1}{x^2}+\frac{1}{x^3}=343$$
$$x^3+3x+3\frac{1}{x}+\frac{1}{x^3}=343$$
$$x^3+3(x+\frac{1}{x})+\frac{1}{x^3}=343$$
$$x^3+21+\frac{1}{x^3}=322$$


**Problem 134**: To solve we know that for $x+\frac{1}{x}=integer$ that the solution for $x^2+\frac{1}{x^2}=integer^2-2$. We can also find that $x^n+\frac{1}{x^n}=(x^{n-1}+\frac{1}{x^{n-1}})(x+\frac{1}{x})-(x^{n-2}+\frac{1}{x^{n-2}})$. And since we know $x+\frac{1}{x}$ and $x^{n-1}+\frac{1}{x^{n-1}}$ and $x^{n-2}+\frac{1}{x^{n-2}}$ are all integers so $x^n+\frac{1}{x^n}$ also must be an integer.

**Problem 135**: If you do couple more, for example:
$$\frac{1}{1+\frac{1}{1+\frac{1}{1+\frac{1}{1+\frac{1}{x}}}}}=\frac{1}{1+\frac{2x+1}{3x+2}}=\frac{1}{\frac{5x+3}{3x+2}}=\frac{3x+2}{5x+3}$$

From this you can see that the coeffeicients of $x$ is the $Fibonacci$ $numbers$.



