# Lecture 1: Integers and the Binary System 

---

## 1. Natural Numbers

The sequence of **natural numbers** is:
\[
0,1,2,3,4,5,6,7,8,9,10,11,\dots
\]

We define:

- **Addition**: $a+b$ is the union of $a$ apples and $b$ apples.  
- **Multiplication**: $a \cdot b$ is the stack of $a$ rows of $b$ apples.  

**Example:**  

- Let $a=2$ â†’ ðŸ”µ ðŸ”µ  
- Let $b=3$ â†’ ðŸŸ¢ ðŸŸ¢ ðŸŸ¢  

Then:
- $a+b$ is  

  ðŸ”µ ðŸ”µ   ðŸŸ¢ ðŸŸ¢ ðŸŸ¢  
- $a \cdot b$ is  

  ðŸ”µ ðŸ”µ ðŸ”µ  
  ðŸ”µ ðŸ”µ ðŸ”µ  

---

### Note
Here we only define **addition** and **multiplication**.  
Subtraction and division are the inverse processes and are omitted.

---

### Basic Laws of Arithmetic

Euler suggested using $a,b,c,\dots$ for specific numbers (and $x,y,z,\dots$ for unknowns). This is the essence of **algebra**.  

The natural numbers satisfy the following laws:

- **Commutative Laws**
  - $a+b=b+a$
  - $ab=ba$

- **Associative Laws**
  - $(a+b)+c=a+(b+c)$
  - $(ab)c=a(bc)$

- **Distributive Laws**
  - $a(b+c)=ab+ac$
  - $(a+b)c=ac+bc$

---

### Proof of Commutativity (Intuitive)

Take:

- $a=2$ â†’ ðŸ”µ ðŸ”µ  
- $b=3$ â†’ ðŸŸ¢ ðŸŸ¢ ðŸŸ¢  

Then:

- $a+b$ = ðŸ”µ ðŸ”µ ðŸŸ¢ ðŸŸ¢ ðŸŸ¢  
- $b+a$ = ðŸŸ¢ ðŸŸ¢ ðŸŸ¢ ðŸ”µ ðŸ”µ  

Clearly, $a+b=b+a$.  

For multiplication:

- $a \cdot b =$  

  ðŸ”µ ðŸ”µ ðŸ”µ  
  ðŸ”µ ðŸ”µ ðŸ”µ  

- $b \cdot a =$  

  ðŸ”µ ðŸ”µ  
  ðŸ”µ ðŸ”µ  
  ðŸ”µ ðŸ”µ  

Thus $ab=ba$. âœ…  

---

### Comments

- **Commutative** and **associative** laws mean the order of operations does not matter:  
  \[
  (4 \cdot 156)\cdot 25=25\cdot (4\cdot 156)=(25\cdot 4)\cdot 156=15600
  \]

- **Distributive law** is helpful for mental arithmetic:  
  \[
  8\cdot 127 = 8\cdot (125+2) = 1000+16 = 1016
  \]

- The second distributive law follows from the first and commutativity:  
  \[
  (a+b)c=c(a+b)=ca+cb=ac+bc
  \]

---

### Decimal System

Using addition and multiplication, we can rigorously define base-$10$:  

\[
756=7\cdot 100+5\cdot 10+6
\]

This makes **vertical calculations** possible.

---

## 2. Binary System

We use base $10$ because we have ten fingers.  
Imagine a world with **two-fingered people** â†’ they would create the **binary system**:

$$0, 1, 10, 11, 100, 101, 110, 111, 1000, 1001, 1010, 1011, ...$$


This corresponds to natural numbers in base $2$.  
For example:
\[
(1011)_2 = 1\cdot 2^3 + 0\cdot 2^2 + 1\cdot 2^1 + 1\cdot 2^0 = 11_{10}
\]

---

### Conversion from Decimal to Binary

Convert $11_{10}$:  

- $11=2\cdot 5+1$  
- $5=2\cdot 2+1$  
- $2=2\cdot 1+0$  
- $1=1$  

Reading remainders upward: $1011_2$.  

---

### Binary Arithmetic

- **Addition**
  - $11+11=110$
  - $111+111=1110$

- **Multiplication**
  - $11\cdot 10=110$
  - $11\cdot 111=10001$

- **Subtraction**
  - $10000-101=1011$

- **Division**
  - $1001/11=11$ (so $1001$ is not prime in binary)  
  - $1/11=0.010101\dots$

ðŸ‘‰ Verify each case against decimal arithmetic.  

---

## 3. Natural Numbers via Peano Axioms

A formal definition avoids dependence on fingers or aliens.  

- $0$ is a natural number.  
- For every $a$, $S(a)$ (the **successor**) is a natural number.  
- If $S(a)=S(b)$, then $a=b$.  
- $S(a)\neq 0$.  

Thus:
\[
1=S(0), \quad 2=S(1)=S(S(0)), \quad \dots
\]

**Addition** is defined recursively:  
- $a+0=a$  
- $a+S(b)=S(a+b)$  
---

**Lemma 1.** $a+S(0)=S(a)$; in other words, $a+1=S(a)$.  

---

**Lemma 2.** $0+b=b$  

**Proof.**  
- $0+0=0$ (definition).  
- $0+1=0+S(0)=S(0+0)=S(0)=1$.  
- $0+2=0+S(1)=S(0+1)=S(1)=2$.  
- Continue forever. âœ…  

---

**Lemma 3.** $S(a)+b=S(a+b)$  

**Proof.**  
- $S(a)+0=S(a)=S(a+0)$.  
- $S(a)+1=S(a)+S(0)=S(S(a)+0)=S(S(a))=S(a+1)$.  
- $S(a)+2=S(a)+S(1)=S(S(a)+1)=S(S(a+1))=S(a+2)$.  
- Continue forever. âœ…  

---

**Theorem.** (Commutativity of Addition)  
\[
a+b=b+a
\]

**Proof.**  
1. **Base case**: $a+0=a=0+a$ (by Lemma 2).  
2. $a+1=a+S(0)=S(a+0)=S(a)=S(0)+a=1+a$.  
3. $a+2=a+S(1)=S(a+1)=S(1+a)=S(1)+a=2+a$.  
4. $a+3=a+S(2)=S(a+2)=S(2+a)=S(2)+a=3+a$.  

By continuing, $a+b=b+a$ for all $b$. âœ…  

> ðŸ’¡ **Note:** This is essentially a **proof by induction**:  
> - Base case: $a+0=0+a$  
> - Inductive step: if $a+b=b+a$, then  
>   \[
>   a+S(b)=S(a+b)=S(b+a)=S(b)+a
>   \]  
> We presented it with small cases for intuition.  

---

<!--
## 9. Negative Numbers (Preview)

- Define $-a$ as $(-1)\cdot a$.  
- Enforcing distributivity:  
  \[
  (-a)+a=(-1)\cdot a+1\cdot a=(-1+1)a=0
  \]
- What about $(-1)(-1)$?  
  \[
  (-1)(-1)+1(-1)=(-1+1)1=0
  \]  
  Since $1(-1)=-1$, it follows $(-1)(-1)=1$.
-->