## Lecture 10: Factorization and Roots
### Factorization: More Difficult Problems

* 

$$
    \begin{align*}
    &x(y^2 - z^2) + y(z^2 - x^2) + z(x^2 - y^2) \\
    &= xy^2 - xz^2 + yz^2 - yx^2 + zx^2 - zy^2 \\
    &= x(y^2 - z^2) + y(z^2 - x^2) + z(x^2 - y^2) \\
    &= x(y - z)(y + z) + y(z - x)(z + x) + z(x - y)(x + y) \\
    &= (y - z)\left[x(y + z) - y(z + x) + z(x + y)\right] \\
    &= (y - z)(y - x)(x - z)
    \end{align*}
    $$

* $$
    \begin{align*}
    a^{10} + a^5 + 1 &= (a^2 + a + 1)\left(a^8 - a^7 + a^5 - a^4 + a^3 - a + 1\right)
    \end{align*}
    $$

* 
    $$
    \begin{align*}
    a^3 + b^3 + c^3 - 3abc &= (a + b + c)\left(a^2 + b^2 + c^2 - ab - bc - ca\right)
    \end{align*}
    $$

* 
    $$
    \begin{align*}
    (a + b + c)^3 - a^3 - b^3 - c^3 &= 3(a^2b + ab^2 + a^2c + ac^2 + b^2c + bc^2 + 2abc) \\
    &= 3\left[a^2(b + c) + a(b^2 + c^2 + 2bc) + bc(b + c)\right] \\
    &= 3(b + c)\left[a^2 + ab + ac + bc\right] \\
    &= 3(a + b)(a + c)(b + c)
    \end{align*}
    $$

* 
    $$
    \begin{align*}
    &a^3 - 3a^2b + 3ab^2 - b^3 + b^3 - 3b^2c + 3bc^2 - c^3 + c^3 - 3c^2a + 3ca^2 - a^3 \\
    &= -3a^2b + 3ab^2 - 3b^2c + 3bc^2 + 3a^2c - 3ac^2 \\
    &= -3(a^2b - ab^2 + b^2c - bc^2 - a^2c + ac^2) \\
    &= -3\left[a^2(b - c) - a(b^2 - c^2) + bc(b - c)\right] \\
    &= -3\left[a^2(b - c) - a(b - c)(b + c) + bc(b - c)\right] \\
    &= -3(b - c)\left[a^2 - ab - ac + bc\right] \\
    &= -3(b - c)(a - b)(a - c)
    \end{align*}
    $$



**Problem 133**: If $x+\frac{1}{x}=7$, calculate
* $x^2+\frac{1}{x^2}=$
$$x+\frac{1}{x}=7$$
$$x^2+2\cdot x \cdot \frac{1}{x}+\frac{1}{x^2}=49$$
$$x^2+2+\frac{1}{x^2}=49$$
$$x^2+\frac{1}{x^2}=47$$
* $x^3+\frac{1}{x^3}=$

$$x^3+3x^2\cdot \frac{1}{x}+3x\cdot \frac{1}{x^2}+\frac{1}{x^3}=343$$
$$x^3+3x+3\frac{1}{x}+\frac{1}{x^3}=343$$
$$x^3+3(x+\frac{1}{x})+\frac{1}{x^3}=343$$
$$x^3+21+\frac{1}{x^3}=322$$

### Roots
**Definition** The $n$-th root of a nonnegative number $a$ is the nonnegative number whose $n$-th power is $a$, denoted by $\sqrt[n]{a}$.


**Example**
* $\sqrt{9}=3$
* $\sqrt[3]{64}=4$
* we may even define the odd roots for negative numbers, $\sqrt[3]{-64}=-4$. But not for even roots.
* Which one is larger? $\sqrt[3]{3}$ or $\sqrt[4]{4}$. Try taking $12$th power.
    *  $(\sqrt[3]{3})^{12}=((\sqrt[3]{3})^{3})^4=81$
    *  $(\sqrt[4]{4})^{12}=((\sqrt[4]{4})^{4})^3=64$
    * So $\sqrt[3]{3}$ is larger.

**Observation**: $(a^{\frac{1}{n}})^n=a$. So $\sqrt[n]{a}=a^{\frac{1}{n}}$.

**Power rules** still hold for fractional numbers $m,n$:
* $a^ma^n=a^{m+n}$
* $(a^m)^n=a^{mn}$
* $a^{-n}=\frac{1}{a^n}$

**Fraction power**: $a^{\frac{m}{n}}=(a^{\frac{1}{n}})^m=\sqrt[n]{a^m}=(\sqrt[n]{a})^m$.

**Example**
* $a^{\frac{2}{3}}a^{\frac{3}{4}}=a^{\frac{2}{3}+\frac{3}{4}}=a^{\frac{17}{12}}$

**Non-fracitonal powers?** How to define $2^{\sqrt{2}}$?
Since ${\sqrt{2}}=1.414...$, we can define a series of powers:
* $2^{1.4}$
* $2^{1.41}$
* $2^{1.414}$
* ...
This series will give us the "limit" number which is $2^{\sqrt{2}}$. This requires calculus to define it. 

**Awesome proof on $\sqrt{2}^{\sqrt{2}}$**
**Theorem:** There exist an irrational power of an irrational number which is rational.

**Proof**: If $\sqrt{2}^{\sqrt{2}}$ is rational, then it is proved. If not, then $\sqrt{2}^{\sqrt{2}}$ is irrational. Now consider
$$(\sqrt{2}^{\sqrt{2}})^{\sqrt{2}}=\sqrt{2}^{\sqrt{2}\sqrt{2}}=\sqrt{2}^2=2.$$
So either $\sqrt{2}^{\sqrt{2}}$ is rational or $(\sqrt{2}^{\sqrt{2}})^{\sqrt{2}}$ is rational. 

**Theorem is proved without knowing the rationality of $\sqrt{2}^{\sqrt{2}}$!!**






